vector-based substitution

theories/lang/lang.v
@@ -163,6 +163,17 @@ Fixpoint subst_l (xl : list binder) (esl : list expr) (e : expr) : option expr :
   | _, _ => None
   end.
 
+Definition subst_l_vec {n} (xl : vec binder n) (el : vec expr n) : expr → expr :=
+  Vector.rect2 (λ _ _ _, expr → expr) id
+               (λ n _ _ rec x e, rec ∘ subst' x e) xl el.
+
+Lemma subst_l_vec_eq {n} (xl : vec binder n) (el : vec expr n) e :
+  Some $ subst_l_vec xl el e = subst_l xl el e.
+Proof.
+  revert n xl el e. eapply (vec_rect2 (λ n xl el, ∀ e, Some $ subst_l_vec xl el e = subst_l xl el e)); first done.
+  move=>n xl el IH x es e. simpl. apply IH.
+Qed.
+
 (** The stepping relation *)
 Definition lit_of_bool (b : bool) : base_lit :=
   LitInt (if b then 1 else 0).
